riscv aspec: rename kernelBase to kernelELFBase and update address space layout comment

spec/machine/RISCV64/Platform.thy
@@ -27,45 +27,59 @@ abbreviation (input) "toPAddr \<equiv> id"
 abbreviation (input) "fromPAddr \<equiv> id"
 
 (* Address space layout:
+The top half of the address space is reserved for the kernel. This means that 256 top level
+entries are for the user, and 256 are for the kernel. This will be further split into the
+'regular' kernel window, which contains mappings to physical memory, a small (1GiB) higher
+kernel image window that we use for running the actual kernel from and a top 1GiB window for
+kernel device mappings. This means that between PPTR_BASE and
+KERNEL_BASE there are 254 entries remaining, which represents how much physical memory
+can be used.
 
-+-----------------------------+ 2^64
-|        Kernel Devices       |
-+-------------------PPTR_KDEV-+ 2^64 - 1GiB
-|         Kernel ELF          |
-+-----------------KERNEL_BASE-+ --+ 2^64 - 2GiB
-|                             |   |
-|                             |   |
-|                             |   |
-|           PSpace            |   |
-|  (direct kernel mappings)   |   +----+
-|                             |   |    |
-|                             |   |    |
-|                             |   |    |
-|                             |   |
-+-------------------PPTR_BASE-+ --+ 2^64 - 2^c
-|                             |                  +-------------------------+
-|                             |        |         |                         |
-|          Invalid            |        |         |                         |
-|      (not canonical)        |        |         |           not           |
-|                             |        |         |         kernel          |
-|                             |        |         |       addressable       |
-+-----------------------------+  2^c   |         |                         |
-|                             |        |         |                         |
-|                             |        |         |                         |
-|                             |        |      +- --------------------------+  PADDR_TOP =
-|                             |        |      |  |                         |  KERNEL_BASE - PPTR_BASE
-|                             |        |      |  |                         |
-|                             |        |      |  |                         |
-|            User             |        |      |  |                         |
-|                             |        |      |  |                         |
-|                             |        +------+  +-------------------------+  PADDR_LOAD + 1GiB
-|                             |     kernel    |  |        Kernel ELF       |
-|                             |   addressable |  +-------------------------+  PADDR_LOAD
-|                             |               |  |                         |
-|                             |               |  |                         |
-+-----------------------------+  0            +- +-------------------------+  0 PADDR_BASE
+Almost all of the top 256 kernel entries will contain 1GiB page mappings. The only 2 entries
+that contain a 2nd level PageTable consisting of 2MiB page entries is the entry
+for the 1GiB Kernel ELF region and the 1GiB region corresponding to the physical memory
+of the kernel ELF in the kernel window.  The same 2nd level PageTable is used and so both
+entries refer to the same 1GiB of physical memory.
+This means that the 1GiB kernel ELF mapping will correspond to physical memory with a 1GiB
+alignment.
 
-  virtual address space                          physical address space
+                  +-----------------------------+ 2^64
+                  |        Kernel Devices       |
+               -> +-------------------PPTR_KDEV-+ 2^64 - 1GiB
+               |  |         Kernel ELF          |
+           ----|  +-------------KERNEL_ELF_BASE-+ --+ 2^64 - 2GiB + (PADDR_LOAD % 1GiB)
+           |   |  |                             |
+           |   -> +-----------------KERNEL_BASE-+ --+ 2^64 - 2GiB
+Shared 1GiB|      |                             |   |
+table entry|      |           PSpace            |   |
+           |      |  (direct kernel mappings)   |   +----+
+           ------>|                             |   |    |
+                  |                             |   |    |
+                  +-------------------PPTR_BASE-+ --+ 2^64 - 2^c
+                  |                             |        |         +-------------------------+
+                  |                             |        |         |                         |
+                  |                             |        |         |                         |
+                  |          Invalid            |        |         |                         |
+                  |                             |        |         |           not           |
+                  |                             |        |         |         kernel          |
+                  |                             |        |         |       addressable       |
+                  +-----------------------------+  2^c   |         |                         |
+                  |                             |        |         |                         |
+                  |                             |        |         |                         |
+                  |                             |        |      +- --------------------------+  PADDR_TOP =
+                  |                             |        |      |  |                         |    KERNEL_BASE - PPTR_BASE
+                  |                             |        |      |  |                         |
+                  |                             |        |      |  |                         |
+                  |            User             |        |      |  |                         |
+                  |                             |        |      |  |                         |
+                  |                             |        +------+  +-------------------------+  PADDR_HIGH_TOP =
+                  |                             |     kernel    |  |        Kernel ELF       |    (PPTR_KDEV - KERNEL_ELF_BASE + PADDR_LOAD)
+                  |                             |   addressable |  +-------------------------+  PADDR_LOAD
+                  |                             |               |  |                         |
+                  |                             |               |  |                         |
+                  +-----------------------------+  0            +- +-------------------------+  0 PADDR_BASE
+
+                     virtual address space                          physical address space
 
 
 c = one less than number of bits the page tables can translate
@@ -78,12 +92,12 @@ definition canonical_bit :: nat
   where
   "canonical_bit = 38"
 
-definition kernelBase :: word64
+definition kernelELFBase :: word64
   where
-  "kernelBase = - (1 << 31) + 0x4000000" (* 2^64 - 2 GiB + 2^26 *)
+  "kernelELFBase = - (1 << 31) + 0x4000000" (* 2^64 - 2 GiB + 2^26 *)
 
-lemma "kernelBase = 0xFFFFFFFF84000000" (* Sanity check with C *)
-  by (simp add: kernelBase_def)
+lemma "kernelELFBase = 0xFFFFFFFF84000000" (* Sanity check with C *)
+  by (simp add: kernelELFBase_def)
 
 definition paddrLoad :: word64
   where
@@ -91,7 +105,7 @@ definition paddrLoad :: word64
 
 definition kernelBaseOffset :: word64
   where
-  "kernelBaseOffset = kernelBase - paddrLoad"
+  "kernelBaseOffset = kernelELFBase - paddrLoad"
 
 definition pptrBase :: word64
   where
